Admit everything

LabeledSeqNum.v
@@ -7,71 +7,70 @@ Section LabeledSeqNum.
   Context {orig_base_params : BaseParams}.
   Context {orig_lb_multi_params : LabeledMultiParams orig_base_params}.
 
-  Record lb_seq_num_data := mkseq_num_data { tdNum  : nat;
-                                             tdSeen : lb_name -> list nat;
-                                             tdData : data }.
+  Record seq_num_data := mkseq_num_data { tdNum  : nat;
+                                          tdSeen : lb_name -> list nat;
+                                          tdData : data }.
 
-  Record lb_seq_num_msg := mkseq_num_msg { tmNum : nat;
-                                           tmMsg : lb_msg }.
+  Record seq_num_msg := mkseq_num_msg { tmNum : nat;
+                                        tmMsg : lb_msg }.
 
-  Definition lb_seq_num_msg_eq_dec (x y : lb_seq_num_msg) : {x = y} + {x <> y}.
+  Definition seq_num_msg_eq_dec (x y : seq_num_msg) : {x = y} + {x <> y}.
     decide equality.
     apply lb_msg_eq_dec.
     decide equality.
   Defined.
 
-  Fixpoint lb_processPackets (seq_num : nat) (packets : list (name * msg)) : nat * list (name * lb_seq_num_msg) :=
+  Fixpoint processPackets (seq_num : nat) (packets : list (name * msg)) : nat * list (name * seq_num_msg) :=
     match packets with
       | [] => (seq_num, [])
-      | p :: ps => let (n', pkts) := lb_processPackets seq_num ps in
+      | p :: ps => let (n', pkts) := processPackets seq_num ps in
                    (n' + 1, (fst p, mkseq_num_msg n' (snd p)) :: pkts)
     end.
 
-
-  Definition lb_seq_num_init_handlers (n : name) :=
+  Definition seq_num_init_handlers (n : name) :=
     mkseq_num_data 0 (fun _ => []) (init_handlers n).
 
-  Definition lb_seq_num_net_handlers
+  Definition seq_num_net_handlers
              (dst : lb_name)
              (src : lb_name)
-             (m : lb_seq_num_msg)
-             (state : lb_seq_num_data) :
-    label * (list output) * lb_seq_num_data * list (name * lb_seq_num_msg) :=
+             (m : seq_num_msg)
+             (state : seq_num_data) :
+    label * (list output) * seq_num_data * list (name * seq_num_msg) :=
     if (member (tmNum m) (tdSeen state src)) then
       (label_silent, [], state, [])
     else
       let '(l,out, data', pkts) := (lb_net_handlers dst src (tmMsg m) (tdData state)) in
-      let (n', tpkts) := lb_processPackets (tdNum state) pkts in
+      let (n', tpkts) := processPackets (tdNum state) pkts in
       (l, out, mkseq_num_data n' (update name_eq_dec (tdSeen state) src (tmNum m :: tdSeen state src)) data', tpkts).
 
-  Definition lb_seq_num_input_handlers
+  Definition seq_num_input_handlers
              (h : name)
              (inp : input)
-             (state : lb_seq_num_data) :
-    label * (list output) * lb_seq_num_data * list (name * lb_seq_num_msg) :=
+             (state : seq_num_data) :
+    label * (list output) * seq_num_data * list (name * seq_num_msg) :=
     let '(l, out, data', pkts) := (lb_input_handlers h inp (tdData state)) in
-    let (n', tpkts) := lb_processPackets (tdNum state) pkts in
+    let (n', tpkts) := processPackets (tdNum state) pkts in
     (l, out, mkseq_num_data n' (tdSeen state) data', tpkts).
 
   Instance base_params : BaseParams :=
     {
-      data := lb_seq_num_data ;
+      data := seq_num_data ;
       input := input ;
       output := output
     }.
 
-  Instance lb_multi_params : LabeledMultiParams _ :=
+  Instance lb_multi_params : LabeledMultiParams base_params :=
     {
       lb_name := lb_name ;
-      lb_msg  := lb_seq_num_msg ;
-      lb_msg_eq_dec := lb_seq_num_msg_eq_dec ;
+      lb_msg  := seq_num_msg ;
+      lb_msg_eq_dec := seq_num_msg_eq_dec ;
       lb_name_eq_dec := lb_name_eq_dec ;
       lb_nodes := lb_nodes ;
       label := label ;
       label_silent := label_silent;
-      lb_init_handlers := lb_seq_num_init_handlers ;
-      lb_net_handlers := lb_seq_num_net_handlers ;
-      lb_input_handlers := lb_seq_num_input_handlers ;
+      lb_init_handlers := seq_num_init_handlers ;
+      lb_net_handlers := seq_num_net_handlers ;
+      lb_input_handlers := seq_num_input_handlers ;
     }.
   Proof.
     - eauto using all_names_nodes.
